Continue with preservation

language_formalisation/type_system/subtyping.v
@@ -1,10 +1,12 @@
-Add LoadPath "C:\Users\Ziga\Documents\Ziga_podatki\PHD\language_formalisation\syntax".
+(* Add LoadPath "C:\Users\Ziga\Documents\Ziga_podatki\PHD\language_formalisation\syntax". *)
+Add LoadPath "E:\Ziga_Podatki\faks\PHD\language_formalisation\syntax".
 Require Import syntax.
 
 
 Inductive vsubtype : vtype -> vtype -> Prop :=
 | VsubtyUnit : vsubtype TyUnit TyUnit
 | VsubtyInt : vsubtype TyInt TyInt
+| VsubtyTyØ : vsubtype TyØ TyØ
 | VsubtyTyΣ A A' B B' : 
     vsubtype A A' -> vsubtype B B' -> vsubtype (TyΣ A B) (TyΣ A' B')
 | VsubtyTyΠ A A' B B' : 
@@ -16,13 +18,19 @@ Inductive vsubtype : vtype -> vtype -> Prop :=
 
 with csubtype : ctype -> ctype -> Prop  :=
 | Csubty A A' Σ Σ' E : 
-    vsubtype A A' -> sigsubtype Σ Σ' -> csubtype (CTy A Σ E) (CTy A' Σ' E)
+    vsubtype A A' -> sig_subtype Σ Σ' -> csubtype (CTy A Σ E) (CTy A' Σ' E)
 
-with sigsubtype : sig -> sig -> Prop :=
-| Σsubty Σ Σ':
-    (forall op A B A' B', (get_op_type Σ op = Some (A, B) -> 
-      (get_op_type Σ' op = Some (A', B')) /\ vsubtype A' A /\ vsubtype B B'))
-    -> sigsubtype Σ Σ'
+with sig_subtype : sig -> sig -> Prop :=
+| SigØsubty : sig_subtype SigØ SigØ
+| SigUsubty Σ Σ' op A B A' B' : 
+    sig_subtype Σ Σ' -> vsubtype A' A -> vsubtype B B' ->
+    sig_subtype (SigU Σ op A B) (SigU Σ' op A' B')
+.
+
+Inductive ctx_subtype : ctx -> ctx -> Prop :=
+| CtxØsubty : ctx_subtype CtxØ CtxØ
+| CtxUsubty Γ Γ' A A' : 
+    ctx_subtype Γ Γ' -> vsubtype A A' -> ctx_subtype (CtxU Γ A) (CtxU Γ' A')
 .
 
 Ltac inv H := inversion H; clear H; subst.
@@ -36,13 +44,15 @@ with csubtype_trans C1 C2 C3
   (C12 : csubtype C1 C2) {struct C12} : csubtype C2 C3 -> csubtype C1 C3
 with csubtype_trans_rev C1 C2 C3 
   (C21 : csubtype C2 C1) {struct C21} : csubtype C3 C2 -> csubtype C3 C1
-with sigsubtype_trans Σ1 Σ2 Σ3 
-  (S12 : sigsubtype Σ1 Σ2) {struct S12} : sigsubtype Σ2 Σ3 -> sigsubtype Σ1 Σ3
-with sigsubtype_trans_rev Σ1 Σ2 Σ3
-  (S21 : sigsubtype Σ2 Σ1) {struct S21} : sigsubtype Σ3 Σ2-> sigsubtype Σ3 Σ1.
+with sig_subtype_trans Σ1 Σ2 Σ3 
+  (S12 : sig_subtype Σ1 Σ2) {struct S12} : sig_subtype Σ2 Σ3 -> 
+  sig_subtype Σ1 Σ3
+with sig_subtype_trans_rev Σ1 Σ2 Σ3
+  (S21 : sig_subtype Σ2 Σ1) (S32 : sig_subtype Σ3 Σ2) {struct S21} : 
+  sig_subtype Σ3 Σ1.
 Proof.
 {
-clear sigsubtype_trans sigsubtype_trans_rev.
+clear sig_subtype_trans sig_subtype_trans_rev.
 intros A23; destruct A12; try assumption; inv A23.
 + apply VsubtyTyΣ.
   - eapply vsubtype_trans. exact A12_1. assumption.
@@ -57,7 +67,7 @@ intros A23; destruct A12; try assumption; inv A23.
   - eapply csubtype_trans_rev. exact H. assumption. 
   - eapply csubtype_trans. exact H0. assumption.
 }{
-clear sigsubtype_trans sigsubtype_trans_rev.
+clear sig_subtype_trans sig_subtype_trans_rev.
 intros A32; destruct A21; try assumption; inv A32.
 + apply VsubtyTyΣ.
   - eapply vsubtype_trans_rev. exact A21_1. assumption.
@@ -72,30 +82,59 @@ intros A32; destruct A21; try assumption; inv A32.
   - eapply csubtype_trans. exact H. assumption. 
   - eapply csubtype_trans_rev. exact H0. assumption.
 }{
-clear vsubtype_trans_rev csubtype_trans csubtype_trans_rev sigsubtype_trans_rev.
+clear vsubtype_trans_rev csubtype_trans csubtype_trans_rev sig_subtype_trans_rev.
 intros C23; destruct C12. inv C23.
 apply Csubty.
 - eapply vsubtype_trans. exact H. assumption.
-- eapply sigsubtype_trans. exact H0. assumption.
+- eapply sig_subtype_trans. exact H0. assumption.
 }{
-clear vsubtype_trans csubtype_trans csubtype_trans_rev sigsubtype_trans.
+clear vsubtype_trans csubtype_trans csubtype_trans_rev sig_subtype_trans.
 intros C32; destruct C21. inv C32.
 apply Csubty.
 - eapply vsubtype_trans_rev. exact H. assumption.
-- eapply sigsubtype_trans_rev. exact H0. assumption.
+- eapply sig_subtype_trans_rev. exact H0. assumption.
 }{
-clear vsubtype_trans vsubtype_trans_rev.
 clear csubtype_trans csubtype_trans_rev.
-clear sigsubtype_trans sigsubtype_trans_rev.
-intros S23; destruct S12. inv S23.
-apply Σsubty. intros.
-apply H0. eapply H in H1. destruct H1. exact H1.
+clear sig_subtype_trans_rev.
+intros S23. destruct S12. inv S23.
+apply SigØsubty.
+inv S23. apply SigUsubty. 
++ eapply sig_subtype_trans. exact S12. assumption.
++ eapply vsubtype_trans_rev. exact H. assumption.
++ eapply vsubtype_trans. exact H0. assumption.
 }{
-clear vsubtype_trans vsubtype_trans_rev.
 clear csubtype_trans csubtype_trans_rev.
-clear sigsubtype_trans sigsubtype_trans_rev.
-intros S32; destruct S21. inv S32.
-apply Σsubty. intros.
-apply H. eapply H0 in H1. destruct H1. exact H1.
+clear sig_subtype_trans.
+destruct S21. inv S32.
+apply SigØsubty.
+inv S32. apply SigUsubty. 
++ eapply sig_subtype_trans_rev. exact S21. assumption.
++ eapply vsubtype_trans. exact H. assumption.
++ eapply vsubtype_trans_rev. exact H0. assumption.
+}
+Qed.
+
+
+Lemma vsubty_refl v : vsubtype v v
+with csubty_refl c : csubtype c c
+with sigsubty_refl Σ : sig_subtype Σ Σ
+with ctx_subty_refl Γ : ctx_subtype Γ Γ.
+Proof.
+{induction v.
++ apply VsubtyUnit.
++ apply VsubtyInt.
++ apply VsubtyTyØ.
++ apply VsubtyTyΣ; assumption.
++ apply VsubtyTyΠ; assumption.
++ apply VsubtyFun. assumption. apply csubty_refl.
++ apply VsubtyHandler; apply csubty_refl.
+}{ destruct c. apply Csubty.
+apply vsubty_refl. apply sigsubty_refl.
+}{ induction Σ.
++ apply SigØsubty.
++ apply SigUsubty; try assumption || apply vsubty_refl.
+}{induction Γ.
++ apply CtxØsubty.
++ apply CtxUsubty. assumption. apply vsubty_refl.
 }
 Qed.
