language_formalisation/type_system/subtyping_lemmas.v
@@ -1,7 +1,74 @@
-Add LoadPath "C:\Users\Ziga\Documents\Ziga_podatki\PHD\language_formalisation\syntax".
-Add LoadPath "C:\Users\Ziga\Documents\Ziga_podatki\PHD\language_formalisation\type_system".
+(* Add LoadPath "C:\Users\Ziga\Documents\Ziga_podatki\PHD\language_formalisation\syntax". *)
+(* Add LoadPath "C:\Users\Ziga\Documents\Ziga_podatki\PHD\language_formalisation\type_system". *)
+Add LoadPath "E:\Ziga_Podatki\faks\PHD\language_formalisation\syntax".
+Add LoadPath "E:\Ziga_Podatki\faks\PHD\language_formalisation\type_system".
+
 Require Import syntax declarational.
 
+Fixpoint ctx_subtype_get Γ Γ' A num
+  (ctx_sty : ctx_subtype Γ Γ') {struct ctx_sty}:
+  get_vtype Γ num = Some A -> 
+  exists A', get_vtype Γ' num = Some A' /\ vsubtype A A'.
+Proof.
+revert num. induction ctx_sty.
++ intros num H. simpl in H. discriminate.
++ intros num get.
+  destruct num.
+  - clear IHctx_sty. simpl in *. injection get. intros. subst. exists A'.
+    constructor. reflexivity. assumption.
+  - simpl in *. eapply IHctx_sty.  clear IHctx_sty. exact get.
+Qed.
+
+Fixpoint ctx_subtype_get_reverse Γ Γ' A num
+  (ctx_sty : ctx_subtype Γ' Γ) {struct ctx_sty}:
+  get_vtype Γ num = Some A -> 
+  exists A', get_vtype Γ' num = Some A' /\ vsubtype A' A.
+Proof.
+revert num. induction ctx_sty.
++ intros num H. simpl in H. discriminate.
++ intros num get.
+  destruct num.
+  - clear IHctx_sty. simpl in *. injection get. intros. subst. exists A0.
+    constructor. reflexivity. assumption.
+  - simpl in *. eapply IHctx_sty.  clear IHctx_sty. exact get.
+Qed.
+
+
+Fixpoint ctx_subtype_vtype Γ Γ' v A:
+  wf_ctx Γ' -> ctx_subtype Γ' Γ -> has_vtype Γ v A -> has_vtype Γ' v A
+with ctx_subtype_ctype Γ Γ' c C:
+  wf_ctx Γ' -> ctx_subtype Γ' Γ -> has_ctype Γ c C -> has_ctype Γ' c C
+with ctx_subtype_htype Γ Γ' h Σ D:
+  wf_ctx Γ' -> ctx_subtype Γ' Γ -> has_htype Γ h Σ D -> has_htype Γ' h Σ D.
+Proof.
+Admitted.
+(* {
+intros wf ctxsty types.
+destruct types. induction H1; apply TypeV; try assumption.
++ apply TypeUnit.
++ apply TypeInt.
++ apply (ctx_subtype_get_reverse _ _ A num) in ctxsty. destruct ctxsty as [A' [gets]]. 
+  eapply TypeVSubtype.
+  - apply TypeV. assumption. apply ctx_gets_wf in gets as wfA'.
+    exact wfA'. assumption. apply TypeVar. assumption.
+  - assumption.
+  - assumption.
++ apply TypePair.
+  - eapply ctx_subtype_vtype. assumption. exact ctxsty. assumption.
+  - eapply ctx_subtype_vtype. assumption. exact ctxsty. assumption.
++ apply TypeInl. admit.
++ admit.
++ apply TypeFun. admit.
++ apply TypeHandler; admit.
++ admit.
+}{
+intros wf ctxsty types.
+destruct types. induction H1; apply TypeC; try assumption.
++ admit.
++ eapply TypeΠMatch.  *)
+
+
+(* ========================== Subtype Shapes ========================== *)
 
 Fixpoint subty_shape_pair A B C :
   vsubtype C (TyΠ A B) -> 
@@ -40,6 +107,9 @@ constructor. reflexivity. constructor; assumption.
 Qed.
 
 
+(* ========================== Value Shapes ========================== *)
+
+(* Pair *)
 Fixpoint shape_pair_full Γ v A B ty (orig : has_vtype Γ v ty) {struct orig} :
   ty = TyΠ A B ->
   (exists name num, v = Var (name, num)) \/
@@ -75,6 +145,8 @@ destruct shape.
 + destruct H as [v1' [v2' [same]]]. injection same. intros. subst. assumption.
 Qed.
 
+
+(* Sum *)
 Fixpoint shape_sum_full Γ v A B ty (orig : has_vtype Γ v ty) {struct orig} :
   ty = TyΣ A B ->
   (exists name num, v = Var (name, num)) \/
@@ -89,7 +161,7 @@ destruct orig. destruct H1; try discriminate.
 + clear shape_sum_full. right. right. exists v. constructor. reflexivity.
   inv same. assumption.
 + rewrite same in H2. apply subty_shape_sum in H2. 
-  destruct H2 as [A'' [B'' [pity]]]. subst. 
+  destruct H2 as [A'' [B'' [sigty]]]. subst. 
   apply (shape_sum_full _ _ A'' B'') in H1. clear shape_sum_full. 
   2: reflexivity. destruct H1.
   - left. assumption.
@@ -126,6 +198,47 @@ destruct shape.
   - destruct H. destruct H. inv H. assumption.
 Qed.
 
+
+(* Function *)
+Fixpoint shape_fun_full Γ v A C ty (orig : has_vtype Γ v ty) {struct orig} :
+  ty = TyFun A C ->
+  (exists name num, v = Var (name, num)) \/
+  (exists x c, v = Fun x c /\ has_ctype (CtxU Γ A) c C).
+Proof.
+intros same.
+destruct orig. destruct H1; try discriminate.
++ clear shape_fun_full. left. exists name. exists num. reflexivity.
++ clear shape_fun_full. right. exists x. exists c. constructor. reflexivity.
+  inv same. assumption.
++ rewrite same in H2. apply subty_shape_fun in H2. 
+  destruct H2 as [A'' [C'' [funty]]]. subst. 
+  apply (shape_fun_full _ _ A'' C'') in H1. clear shape_fun_full. 
+  2: reflexivity. destruct H1.
+  - left. assumption.
+  - right. destruct H1. destruct H1 as [c']. exists x. exists c'.
+    destruct H1. constructor. assumption.
+    apply TypeC; inv H0.
+    * apply WfCtxU; assumption.
+    * assumption.
+    * destruct H2. eapply TypeCSubtype. 2: exact H1.
+      eapply ctx_subtype_ctype. 3: exact H3.
+      apply WfCtxU; assumption.
+      apply CtxUsubty. apply ctx_subty_refl. assumption.
+Qed.
+
+Lemma shape_fun Γ x c A C :
+  has_vtype Γ (Fun x c) (TyFun A C) -> has_ctype (CtxU Γ A) c C.
+Proof.
+intro orig.
+apply (shape_fun_full _ _ A C) in orig as shape. 2: reflexivity.
+destruct shape.
++ destruct H as [name [num]]. discriminate.
++ destruct H. destruct H. destruct H. inv H. inv H0. apply TypeC; assumption.
+Qed.
+
+(* ========================== Computation Shapes ========================== *)
+
+(* ΠMatch *)
 Fixpoint shape_prodmatch_full Γ c v x y c' C
   (orig : has_ctype Γ c C) {struct orig} :
   c = (ΠMatch v (x, y) c') ->
@@ -152,6 +265,8 @@ intro orig. apply (shape_prodmatch_full _ _ v x y c) in orig.
 2: reflexivity. assumption.
 Qed.
 
+
+(* ΣMatch *)
 Fixpoint shape_summatch_full Γ c v xl cl xr cr C
   (orig : has_ctype Γ c C) {struct orig} :
   c = (ΣMatch v xl cl xr cr) ->
@@ -179,5 +294,32 @@ Fixpoint shape_summatch Γ v xl cl xr cr C :
     has_ctype (CtxU Γ A) cl C /\ has_ctype (CtxU Γ B) cr C).
 Proof.
 intro orig. apply (shape_summatch_full _ _ v xl cl xr cr) in orig.
+2: reflexivity. assumption.
+Qed.
+
+
+(* App *)
+Fixpoint shape_app_full Γ c x c' v C
+  (orig : has_ctype Γ c C) {struct orig} :
+  c = (App (Fun x c') v) ->
+  (exists A, has_ctype (CtxU Γ A) c' C /\ has_vtype Γ v A).
+Proof.  
+intros same. destruct orig. destruct H1; try discriminate.
++ clear shape_app_full. 
+  inv same. exists A. apply shape_fun in H1. constructor; assumption.
++ apply (shape_app_full _ _ x c' v) in H1;
+  clear shape_app_full. 2: assumption.
+  destruct H1 as [A' [cty]].
+  exists A'. constructor. 2: assumption.
+  inv cty. apply TypeC; auto.
+  eapply TypeCSubtype. apply TypeC.
+  assumption. exact H4. exact H5. assumption.
+Qed.
+
+Fixpoint shape_app Γ x c v C :
+  has_ctype Γ (App (Fun x c) v) C ->
+  (exists A, has_ctype (CtxU Γ A) c C /\ has_vtype Γ v A).
+Proof.
+intro orig. eapply (shape_app_full _ _ x c v C) in orig.
 2: reflexivity. assumption.
 Qed.
